\documentclass[a4paper,twoside,12pt]{article}
\usepackage{amsfonts}
\begin{document}

Let $ \mathbf{s} = \{ s_1, s_2, ... , s_N \}, \mathbf{\alpha} = \{s_1 + s_2 + ... + s_N \}$ and $\mathbf{\beta} = \{s_1^2 + s_2^2 + ... + s_N^2 \}$ where $\mathbf{s} \in R^N$. Then the mean of $\mathbf{s}$ $\mu = \frac{1}{N} \sum_{i=1}^N{x_i}$ and standard deviation $ \sigma = \sqrt{\frac{1}{N - 1} \sum_{i=1}^N{(x_i - \mu)^2} } $ could be re-written in terms of $\alpha$ and $\beta$ as $ \mu = \mathbf{\alpha} / N$ and $ \sigma = \sqrt{ \frac{\mathbf{\beta} - N\mu^2}{N-1}} $ respectively.

If you want the demonstration then we have to meet in McDonads !

\end{document}